@base             <http://on.cs.unibas.ch/owl/1.0/> .
@prefix      owl: <http://www.w3.org/2002/07/owl#> .
@prefix      xsd: <http://www.w3.org/2001/XMLSchema#> .
@prefix     rdfs: <http://www.w3.org/2000/01/rdf-schema#> .
@prefix      rdf: <http://www.w3.org/1999/02/22-rdf-syntax-ns#> .
@prefix elements: <http://purl.org/dc/elements/1.1/#> .
@prefix  Context: <Context.owl#> .

# Named toplevel resources (37)

<Context.owl>
	a owl:Ontology ;
	elements:creator "Thorsten MÃ¶ller" ;
	elements:date "2010-03-15" ;
	elements:rights "    Copyright 2009-2010 University of Basel Switzerland\n  " ;
	rdfs:comment "    Conceptualization of a generic context model. Its basic notions are\n    DataGenerator (a.k.a. Sensor), Subject, and ContextObject. Their\n    relationships and basic properties are modeled by means of various\n    properties.\n  "@en ;
	owl:versionInfo "    $Id: Context.owl 297 2010-03-15 15:54:36Z thorsten $\n  " .

Context:ContextObject
	a owl:Class ;
	rdfs:comment "\t\tAny context data about a Subject generated/measured by some DataGenerator.\n\t"@en .

Context:DataGenerator
	a owl:Class ;
	rdfs:comment "\t\tGenerates context data by monitoring a subject, which is the 'source' of\n\t\tcontext information.\n\t"@en .

Context:DataMode
	a owl:Class ;
	rdfs:comment "\t\tThe data mode describes whether a DataGenerator generates single non-\n\t\tcontiguous data items or whether it generates a (infinite) sequence of\n\t\tcoherent data items separated by a (equidistant) time interval.\n\t"@en ;
	owl:oneOf ( Context:Single
		    Context:Stream
		  ) .

Context:HardwareSensor
	a owl:Class ;
	rdfs:comment "\t\tA physical device that measures some physical quantity and converts it\n\t\tinto a signal, expressed by means of some continuous or discrete data.\n\t\tFor instance, a digital temperature sensor, or a GPS device.\n\t"@en ;
	rdfs:subClassOf Context:DataGenerator .

Context:Human
	a owl:Class ;
	rdfs:comment "\t\tA human person may act like a data generator manually metering some subject\n\t\tby manually entering data into some software.\n\t\tFor instance, a person that regularly measures its blood pressure manually\n\t\tand enters the values into some software system.\n\t"@en ;
	rdfs:subClassOf Context:DataGenerator ;
	owl:disjointWith Context:HardwareSensor ,
			 Context:SoftwareSensor .

Context:OperationMode
	a owl:Class ;
	rdfs:comment "\t\tA DataGenerator operates either in push or pull mode.\n\t"@en ;
	owl:oneOf ( Context:Push
		    Context:Pull
		  ) .

Context:Pull
	a Context:OperationMode .

Context:Push
	a Context:OperationMode .

Context:Sensor
	a owl:Class ;
	rdfs:comment "\t\tSome thing that measures a physical or virtual quantity and converts it\n\t\tinto a signal. The latter is meant to be data (i.e., not a physical signal).\n\t\tEverything that is a sensor is in particular a data generator and vice versa.\n\t"@en ;
	owl:equivalentClass Context:DataGenerator .

Context:Single
	a Context:DataMode .

Context:SoftwareSensor
	a owl:Class ;
	rdfs:comment "\t\tA piece of software that measures some virtual quantity and converts it\n\t\tinto a signal, expressed by means of some continuous or discrete data.\n\t\tFor instance, some procedure that measures the current load of a CPU.\n\t"@en ;
	rdfs:subClassOf Context:DataGenerator .

Context:Stream
	a Context:DataMode .

Context:Subject
	a owl:Class ;
	rdfs:comment "\t\tSome thing that is subject to be (regularly) measured by some DataGenerator\n\t\trespectively Sensor.\n\t\tNote that it is not disjoint with DataGenerator in order to allow expressing\n\t\tthat a DataGenerator may itself be a Subject for another DataGenerator. For\n\t\tinstance, some person that measures its blood pressure manually (hence, it is\n\t\ta Human DataGenerator), while its heart rhythm is also subject to be measured\n\t\tautomatically by another HardwareSensor (hence, it is also a Subject).\n\t"@en .

Context:about
	a owl:ObjectProperty ;
	rdfs:comment "\t\tContext objects (generated by some DataGenerator) are about some Subject,\n\t\ti.e., (partially) represent its context. See also the \"measures\" property.\n\t"@en ;
	rdfs:domain Context:ContextObject ;
	rdfs:range Context:Subject .

Context:aboutContext
	a owl:ObjectProperty ;
	rdfs:comment "\t\tMore specific meta object property to be used for ContextObjects, which\n\t\tis the reason why the range is limited to ContextObject.\n\t\tThe domain is left unspecified in order to allow creating custom sub\n\t\tproperties.\n\t"@en ;
	rdfs:range Context:ContextObject ;
	rdfs:subPropertyOf Context:metaAbout .

Context:aboutDataGenerator
	a owl:ObjectProperty ;
	rdfs:comment "\t\tMore specific meta object property to be used for DataGenerators, which\n\t\tis the reason why the range is limited to DataGenerator.\n\t\tThe domain is left unspecified in order to allow creating custom sub\n\t\tproperties.\n\t"@en ;
	rdfs:range Context:DataGenerator ;
	rdfs:subPropertyOf Context:metaAbout .

Context:accuracy
	a owl:DatatypeProperty ;
	rdfs:comment "\t\tAccuracy of some quantifiable ContextObject in percent, relative to the\n\t\tmeasured ContextObject value.\n\t\tAccuracy is the degree of veracity (closeness) of a measured ContextObject\n\t\tto its actual (true) value.\n\t"@en ;
	rdfs:range xsd:nonNegativeInteger ;
	rdfs:subPropertyOf Context:contextMetaData .

Context:containedIn
	a owl:ObjectProperty ;
	owl:inverseOf Context:contains .

Context:contains
	a owl:IrreflexiveProperty ,
	  owl:ObjectProperty ,
	  owl:TransitiveProperty ;
	rdfs:comment "\t\tExpresses that a ContextObject consists of another ContextObject, i.e., they\n\t\tcan be either atomic or composite. Furthermore, this property is transitive\n\t\tand irreflexive: if x,y,z are ContextObjects and x contains y and y contains\n\t\tz then x contains z; but x can not contain x (itself).\n\t"@en ;
	rdfs:domain Context:ContextObject ;
	rdfs:range Context:ContextObject .

Context:contextMeta
	a owl:ObjectProperty ;
	rdfs:comment "\t\tMore specific has meta object property to be used for ContextObjects, which\n\t\tis the reason why the domain is limited to ContextObject.\n\t\tThe range is left unspecified in order to allow creating custom sub\n\t\tproperties.\n\t"@en ;
	rdfs:domain Context:ContextObject ;
	rdfs:subPropertyOf Context:hasMeta ;
	owl:inverseOf Context:aboutContext .

Context:contextMetaData
	a owl:DatatypeProperty ;
	rdfs:comment "\t\tMore specific meta data property to be used for ContextObjects, which is\n\t\tthe reason why the domain is limited to ContextObject.\n\t\tThe range is left unspecified in order to allow creating custom sub\n\t\tproperties.\n\t"@en ;
	rdfs:domain Context:ContextObject ;
	rdfs:subPropertyOf Context:hasMetaData .

Context:dataGeneratorMeta
	a owl:ObjectProperty ;
	rdfs:comment "\t\tMore specific has meta object property to be used for DataGenerators,\n\t\twhich\tis the reason why the domain is limited to DataGenerator.\n\t\tThe range is left unspecified in order to allow creating custom sub\n\t\tproperties.\n\t"@en ;
	rdfs:domain Context:DataGenerator ;
	rdfs:subPropertyOf Context:hasMeta ;
	owl:inverseOf Context:aboutDataGenerator .

Context:dataGeneratorMetaData
	a owl:DatatypeProperty ;
	rdfs:comment "\t\tMore specific meta data property to be used for DataGenerators, which\n\t\tis the reason why the domain is limited to DataGenerator.\n\t\tThe range is left unspecified in order to allow creating custom sub\n\t\tproperties.\n\t"@en ;
	rdfs:domain Context:DataGenerator ;
	rdfs:subPropertyOf Context:hasMetaData .

Context:dataMode
	a owl:ObjectProperty ;
	rdfs:domain Context:DataGenerator ;
	rdfs:range Context:DataMode .

Context:frequency
	a owl:DatatypeProperty ;
	rdfs:comment "\t\tFrequency of consecutive and equidistant measurements by a DataGenerator.\n\t\tUnit is Herz.\n\t"@en ;
	rdfs:range xsd:float ;
	rdfs:subPropertyOf Context:dataGeneratorMetaData .

Context:generatedBy
	a owl:FunctionalProperty ,
	  owl:ObjectProperty ;
	rdfs:comment "\t\tExpresses the origin on a ContextObject, i.e., by whom it was generated.\n\t\tFurthermore, this property\tis functional: if x is a ContextObject, a,b\n\t\tare DataGenerators and x was generated by both a and b then a is the same\n\t\tas b.\n\t"@en ;
	rdfs:domain Context:ContextObject ;
	rdfs:range Context:DataGenerator .

Context:hasGenerated
	a owl:ObjectProperty ;
	owl:inverseOf Context:generatedBy .

Context:hasMeta
	a owl:ObjectProperty ;
	rdfs:comment "\t\tThis property is the root of meta object properties of different types.\n\t\tThe intension is to refer the actual meta individual that some individual\n\t\thas, i.e., it is the inverse of the #metaAbout property.\n\t\tSpecific meta object properties will specialize this property by\n\t\trestricting the domain and range appropriately and using\tsubPropertyOf.\n\t"@en ;
	owl:inverseOf Context:metaAbout .

Context:hasMetaData
	a owl:DatatypeProperty ;
	rdfs:comment "\t\tThis property is the root of meta data properties of different types. The\n\t\tintension is to refer the actual meta data value that some individual has.\n\t\tSpecific meta data properties will specialize this property by\n\t\trestricting the domain and range appropriately and using subPropertyOf.\n\t"@en .

Context:measuredBy
	a owl:ObjectProperty ;
	rdfs:comment "\t\tA Subject s with a ContextObject o which was generated by a DataGenerator g\n\t\tis said to be measured by this data generator g.\n\t\tNote that a Subject can be measured/monitored by one or more DataGenerators.\n\t\tAlso note that this is the inverse direction of the measures property.\n\t"@en ;
	owl:inverseOf Context:measures ;
	owl:propertyChainAxiom ( Context:with
				 Context:generatedBy
			       ) .

Context:measures
	a owl:ObjectProperty ;
	rdfs:comment "\t\tA DataGenerator g which has generated a ContextObject o which is about a\n\t\tSubject s is said to be measuring this subject s.\n\t\tNote that a DataGenerator may measure/monitor multiple Subjects.\n\t"@en ;
	owl:propertyChainAxiom ( Context:hasGenerated
				 Context:about
			       ) .

Context:metaAbout
	a owl:ObjectProperty ;
	rdfs:comment "\t\tThis property is the root of meta object properties of different types.\n\t\tIts intension is to refer the individual which some meta individual is\n\t\tabout.\n\t\tSpecific meta object properties will specialize this property by\n\t\trestricting the domain and range appropriately and using subPropertyOf.\n\t"@en .

Context:precision
	a owl:DatatypeProperty ;
	rdfs:comment "\t\tPrecision of some DataGenerator in percent.\n\t\tPrecision is the degree of reproducibility of a measured ContextObject to\n\t\tits actual (true) value, i.e., the degree to which further measurements\n\t\tshow the same or similar results.\n\t"@en ;
	rdfs:range xsd:nonNegativeInteger ;
	rdfs:subPropertyOf Context:dataGeneratorMetaData .

Context:timestamp
	a owl:DatatypeProperty ;
	rdfs:comment "\t\tThe Date and Time when some ContextObject was generated by a Sensor/DataGenerator.\n\t"@en ;
	rdfs:range xsd:dateTime ;
	rdfs:subPropertyOf Context:contextMetaData .

Context:usageMode
	a owl:ObjectProperty ;
	rdfs:domain Context:DataGenerator ;
	rdfs:range Context:OperationMode .

Context:with
	a owl:ObjectProperty ;
	owl:inverseOf Context:about .
